Update.

src/metalogic/fol_mm0.lean
@@ -1612,6 +1612,98 @@ begin
 end
 
 
+def id_instantiation : instantiation := ⟨ id, by simp ⟩
+
+example
+  {D : Type}
+  (V : valuation D)
+  (M : meta_valuation D)
+  (E : env)
+  (τ : meta_instantiation)
+  (φ : formula)
+  (h1 : φ.is_meta_var_or_all_def_in_env E)
+  (h2 : ∀ (X : meta_var_name), X ∈ φ.meta_var_set → (τ X).is_meta_var_or_all_def_in_env E)
+  (h3 : E.nodup_) :
+  (holds D (fun (X' : meta_var_name), holds D M E (τ X')) E φ V
+    ↔ holds D M E (formula.subst id_instantiation τ φ) V) :=
+begin
+  induction φ generalizing V,
+  case formula.meta_var_ : X V
+  {
+    unfold formula.subst,
+    simp only [holds_meta_var],
+  },
+  case formula.not_ : φ φ_ih V
+  {
+    unfold formula.is_meta_var_or_all_def_in_env at h1,
+    unfold formula.subst,
+    simp only [holds_not],
+    apply not_congr,
+    exact φ_ih h1 h2 V,
+  },
+  case formula.imp_ : φ_ᾰ φ_ᾰ_1 φ_ih_ᾰ φ_ih_ᾰ_1 V
+  { admit },
+  case formula.eq_ : φ_ᾰ φ_ᾰ_1 V
+  { admit },
+  case formula.forall_ : φ_ᾰ φ_ᾰ_1 φ_ih V
+  { admit },
+  case formula.def_ : name args V
+  {
+    induction E,
+    case list.nil
+    {
+      unfold formula.is_meta_var_or_all_def_in_env at h1,
+      simp only [list.not_mem_nil, false_and, exists_false] at h1,
+      contradiction,
+    },
+    case list.cons : E_hd E_tl E_ih
+    {
+      have s1 : E_hd.q.meta_var_set = ∅,
+      exact no_meta_var_imp_meta_var_set_is_empty E_hd.q E_hd.args E_hd.nf,
+
+      unfold formula.subst,
+      simp only [holds_meta_var, holds_not_nil_def, list.length_map, list.map_map],
+      split_ifs,
+      {
+        cases h,
+        unfold id_instantiation,
+        simp only [function.comp.right_id],
+        rewrite holds_meta_valuation_ext,
+        rewrite s1,
+        simp only [finset.not_mem_empty, is_empty.forall_iff, forall_forall_const, implies_true_iff],
+      },
+      {
+        unfold formula.is_meta_var_or_all_def_in_env at h1,
+        apply exists.elim h1,
+        intros d h1_1,
+        clear h1,
+        cases h1_1,
+        simp only [list.mem_cons_iff] at h1_1_left,
+
+        cases h1_1_left,
+        {
+          rewrite <- h1_1_left at h,
+          exfalso,
+          apply h,
+          exact h1_1_right,
+        },
+        {
+          unfold id_instantiation,
+          simp only [function.comp.right_id],
+          simp only [list.map_id],
+
+          rewrite <- holds_meta_valuation_ext
+          (fun (X' : meta_var_name), holds D M (E_hd :: E_tl) (τ X'))
+          M E_tl V (def_ name args),
+          unfold formula.meta_var_set,
+          simp only [finset.not_mem_empty, is_empty.forall_iff, forall_forall_const, implies_true_iff],
+        },
+      }
+    },
+  },
+end
+
+
 lemma holds_subst_aux
   {D : Type}
   (V : valuation D)
